Finish the tactic to unfold proj_reptype and upd_reptype (pose_proj_reptype and pose_upd_reptype). Half way of applying them in examples. More automation of zlist is added.

progs/verif_revarray.v
@@ -14,12 +14,12 @@ Definition reverse_spec :=
           PROP (0 <= size <= Int.max_signed;
                 writable_share sh;
                 size = Zlength contents;
-                forall i, 0 <= i < size -> is_int I32 Signed (zl_nth i (contents: reptype_array tint 0 size)))
+                forall i, 0 <= i < size -> is_int I32 Signed (Znth i contents Vundef))
           LOCAL (temp _a a0; temp _n (Vint (Int.repr size)))
-          SEP (`(data_at sh (tarray tint size) contents a0))
+          SEP (`(data_at sh (tarray tint size) (zl_constr tint 0 size contents) a0))
   POST [ tvoid ]
      PROP() LOCAL()
-     SEP(`(data_at sh (tarray tint size) (rev contents) a0)).
+     SEP(`(data_at sh (tarray tint size) (zl_constr tint 0 size (rev contents)) a0)).
 
 Definition main_spec :=
  DECLARE _main
@@ -32,22 +32,24 @@ Definition Vprog : varspecs := (_four, Tarray tint 4 noattr)::nil.
 Definition Gprog : funspecs := 
     reverse_spec :: main_spec::nil.
 
-Definition flip_between {A} lo hi (contents: list A) :=
-  rev (skipn (Z.to_nat hi) contents) ++
-  skipn (Z.to_nat lo) (firstn (Z.to_nat hi) contents) ++
-  rev (firstn (Z.to_nat lo) contents).
+Definition flip_between t lo hi size (contents: list (reptype t)) :=
+  zl_concat (zl_sublist 0 lo (zl_constr t 0 size (rev contents)))
+    (zl_concat (zl_sublist lo hi (zl_constr t 0 size contents))
+                  (zl_sublist hi size (zl_constr t 0 size (rev contents)))).
 
 Definition reverse_Inv a0 sh contents size := 
  EX j:Z,
   (PROP  (0 <= j; j <= size-j; isptr a0;
           size = Zlength contents;
-          forall i, 0 <= i < size -> is_int I32 Signed (zl_nth i (contents: reptype_array tint 0 size)))
+          forall i, 0 <= i < size -> is_int I32 Signed (Znth i contents Vundef))
    LOCAL  (temp _a a0; temp _lo (Vint (Int.repr j)); temp _hi (Vint (Int.repr (size-j))))
-   SEP (`(data_at sh (tarray tint size) (flip_between j (size-j) contents) a0))).
+   SEP (`(data_at sh (tarray tint size) (flip_between tint j (size-j) size contents) a0))).
 
-Lemma flip_fact_0: forall {A} (contents: list A),
-  contents = flip_between 0 (Zlength contents - 0) contents.
+Lemma flip_fact_0: forall t size (contents: list (reptype t)),
+  zl_constr t 0 size contents = flip_between t 0 (size - 0) size contents.
 Proof.
+  admit.
+(*
   intros.
   unfold flip_between.
   rewrite Z.sub_0_r.
@@ -59,13 +61,17 @@ Proof.
   rewrite app_nil_r.
   rewrite firstn_exact_length.
   reflexivity.
+*)
 Qed.
 
-Lemma flip_fact_1: forall {A} (contents: list A) j,
+Lemma flip_fact_1: forall t size (contents: list (reptype t)) j,
   0 <= j ->
-  Zlength contents - j - 1 <= j <= Zlength contents - j ->
-  flip_between j (Zlength contents - j) contents = rev contents.
+  size - j - 1 <= j <= size - j ->
+  flip_between t j (size - j) size contents =
+   zl_constr t 0 size (rev contents).
 Proof.
+  admit.
+(*
   intros.
   assert (Zlength contents - j - 1 = j \/ Zlength contents - j = j)
     by (destruct (zle (Zlength contents - j) j); omega).
@@ -92,8 +98,9 @@ Proof.
     by (apply Z2Nat.inj_le; omega).
   rewrite !firstn_skipn.
   reflexivity.
+*)
 Qed.
-
+(*
 Lemma flip_fact_2: forall {A} (contents: list A) j k d,
   0 <= j <= Zlength contents - j - 1 ->
   j <= k < Zlength contents - j ->
@@ -129,6 +136,7 @@ Proof.
   f_equal.
   omega.
 Qed.
+*)
 
 Lemma body_reverse: semax_body Vprog Gprog f_reverse reverse_spec.
 Proof.
@@ -150,7 +158,7 @@ forward _. (* hi = n; *)
 
 forward_while (reverse_Inv a0 sh contents size)
     (PROP  () LOCAL  (temp _a a0)
-   SEP (`(data_at sh (tarray tint size) (rev contents) a0)))
+   SEP (`(data_at sh (tarray tint size) (zl_constr tint 0 size (rev contents)) a0)))
    j.
 (* Prove that current precondition implies loop invariant *)
 apply exp_right with 0.
@@ -167,15 +175,18 @@ apply derives_refl'.
 f_equal.
 apply flip_fact_1; omega.
 (* Prove that loop body preserves invariant *)
-Opaque zl_nth.
+unfold flip_between.
+Opaque zl_nth zl_concat zl_sublist.
 forward. (* t = a[lo]; *)
 {
   entailer!.
-  specialize (POP j).
-  spec POP; [omega |].
-  rewrite zl_nth_LZ, Z.sub_0_r in POP |- * by omega.
-  rewrite flip_fact_2 by omega.
-  exact POP.
+  rewrite zl_concat_correct by omega.
+  if_tac; [omega |].
+  rewrite zl_concat_correct by omega.
+  if_tac; [| omega].
+  rewrite zl_sublist_correct by omega.
+  rewrite zl_constr_correct by omega.
+  apply POP; omega.
 }
 forward.  (* s = a[hi-1]; *)
 {
