floyd/forward.v
@@ -876,11 +876,36 @@ Proof.
   apply Znth_map.
 Qed.
 
+Lemma zl_concat_correct_l: forall {A} {d} {ZL: Zlist A d} `{@Zlist_Correct _ _ ZL} i lo mid hi (l1 : zlist A lo mid) (l2: zlist A mid hi),
+  lo <= i < mid ->
+  lo <= mid <= hi ->
+  zl_nth i (zl_concat l1 l2) = zl_nth i l1.
+Proof.
+  intros.
+  rewrite zl_concat_correct by omega.
+  if_tac; auto.
+  omega.
+Qed.
+
+Lemma zl_concat_correct_r: forall {A} {d} {ZL: Zlist A d} `{@Zlist_Correct _ _ ZL} i lo mid hi (l1 : zlist A lo mid) (l2: zlist A mid hi),
+  mid <= i < hi ->
+  lo <= mid <= hi ->
+  zl_nth i (zl_concat l1 l2) = zl_nth i l2.
+Proof.
+  intros.
+  rewrite zl_concat_correct by omega.
+  if_tac; auto.
+  omega.
+Qed.
+
 End zlist_hint_db.
 
 Hint Rewrite @zl_constr_correct using solve [omega] : zlist_db.
+Hint Rewrite @zl_sublist_correct using solve [omega] : zlist_db.
 Hint Rewrite zlist_hint_db.Znth_sub_0_r : zlist_db.
 Hint Rewrite zlist_hint_db.Znth_map_Vint using solve [omega] : zlist_db.
+Hint Rewrite @zlist_hint_db.zl_concat_correct_l using solve [omega] : zlist_db.
+Hint Rewrite @zlist_hint_db.zl_concat_correct_r using solve [omega] : zlist_db.
 
 Ltac do_compute_lvalue Delta P Q R e v H :=
   let rho := fresh "rho" in
@@ -2152,11 +2177,19 @@ intros. destruct v; inv H; reflexivity.
 Qed.
 Hint Rewrite sem_add_ptr_int using assumption : norm.
 
-Check semax_SC_field_cast_load.
-
-Ltac unfold_proj' t gfs v :=
-match goal with
-| gfs := ?GFS |- _ => subst gfs; unfold_proj t GFS v
+Ltac solve_load_rule_evaluation :=
+  match goal with
+  | |- repinject _ (@proj_reptype ?cs ?csl ?t ?gfs ?v) = _ =>
+         rewrite (repinject_JMeq _ (@proj_reptype cs csl t gfs v)) by reflexivity;
+         match goal with
+         | gfs := ?gfs' |- _ =>
+           let t' := eval compute in t in
+           let H := fresh "H" in
+           pose_proj_reptype cs csl t' gfs' v H;
+           subst v; autorewrite with zlist_db in H;
+           exact H
+  | _ => idtac
+  end
 end.
 
 Ltac new_load_tac :=   (* matches:  semax _ _ (Sset _ (Efield _ _ _)) _  *)
@@ -2218,7 +2251,7 @@ Ltac new_load_tac :=   (* matches:  semax _ _ (Sset _ (Efield _ _ _)) _  *)
     eapply (semax_SC_field_cast_load Delta sh n) with (lr0 := lr) (t_root0 := t_root) (gfs2 := gfs0) (gfs3 := gfs1);
     [reflexivity | reflexivity | reflexivity
     | reflexivity | exact Heq | exact HLE | exact H_Denote | exact H
-    | unfold_proj' (nested_field_type2 t_root gfs0) gfs1 v; subst v; autorewrite with zlist_db; reflexivity
+    | solve_load_rule_evaluation
     | unfold tc_efield; try solve [entailer!]; try (clear Heq HLE H_Denote H H_LEGAL;
       subst e1 gfs0 gfs1 efs tts t_root v sh lr n; simpl app; simpl typeof)
     | solve_legal_nested_field_in_entailment;
@@ -2283,7 +2316,7 @@ Ltac new_load_tac :=   (* matches:  semax _ _ (Sset _ (Efield _ _ _)) _  *)
     eapply (semax_SC_field_load Delta sh n) with (lr0 := lr) (t_root0 := t_root) (gfs2 := gfs0) (gfs3 := gfs1);
     [reflexivity | reflexivity | reflexivity
     | reflexivity | exact Heq | exact HLE | exact H_Denote | exact H
-    | unfold_proj' (nested_field_type2 t_root gfs0) gfs1 v; subst v; autorewrite with zlist_db; reflexivity
+    | solve_load_rule_evaluation
     | unfold tc_efield; try solve [entailer!]; try (clear Heq HLE H_Denote H H_LEGAL;
       subst e1 gfs0 gfs1 efs tts t_root v sh lr n; simpl app; simpl typeof)
     | solve_legal_nested_field_in_entailment; try clear Heq HLE H_Denote H H_LEGAL;
